theories/soundness/newc.v
@@ -17,7 +17,7 @@ Section proofs.
   (* assume a given set of class definitions *)
   Context `{PDC: ProgDefContext}.
   (* assume some SDT constraints and their properties *)
-  Context `{SDTCP: SDTClassSpec}.
+  Context `{SDTCS: SDTClassSpec}.
 
   (* Helping the inference with this notation that hides pdefs *)
   Local Notation "Δ ⊢ s <: t" := (@subtype _ _ Δ Plain s t) (at level 70, s at next level, no associativity).
